pcuic/theories/PCUICLiftSubst.v
@@ -161,6 +161,15 @@ Fixpoint extended_subst (Γ : context) (n : nat)
     end
   end.
 
+Definition expand_lets_k Γ k t := 
+  (subst (extended_subst Γ 0) k (lift (context_assumptions Γ) (k + #|Γ|) t)).
+
+Definition expand_lets Γ t := expand_lets_k Γ 0 t.
+
+Definition expand_lets_k_ctx Γ k Δ := 
+  (subst_context (extended_subst Γ 0) k (lift_context (context_assumptions Γ) (k + #|Γ|) Δ)).
+
+Definition expand_lets_ctx Γ Δ := expand_lets_k_ctx Γ 0 Δ.
 
 Fixpoint closedn k (t : term) : bool :=
   match t with
